Weaken env_ok requirements on constructors
It's OK that the constructors exist in the constructor environment
(otherwise we cannot pattern match on them, for instance), as long
as they can only be accessed by their original names.

candle/prover/candle_prover_invScript.sml
@@ -121,8 +121,10 @@ Inductive v_ok:
        v_ok ctxt (Env env ns)) ∧
 [env_ok:]
   (∀ctxt env.
-     (∀n len tag m. nsLookup env.c n = SOME (len, TypeStamp tag m) ⇒
-                  m ∉ kernel_types) ∧
+     (∀id len tag tn.
+        nsLookup env.c id = SOME (len, TypeStamp tag tn) ∧
+        tn ∈ kernel_types ⇒
+          id_to_n id ∈ kernel_ctors) ∧
      (∀n v. nsLookup env.v n = SOME v ⇒ v_ok ctxt v) ⇒
        env_ok ctxt env)
 End
@@ -135,7 +137,7 @@ Proof
 QED
 
 Theorem kernel_vals_Env[simp]:
-  ~kernel_vals ctxt1 (Env env id)
+  ¬kernel_vals ctxt1 (Env env id)
 Proof
   rw [Once v_ok_cases]
   \\ gs [do_partial_app_def, CaseEqs ["exp", "v"]]
@@ -320,7 +322,6 @@ Theorem env_ok_with_nsBind:
 Proof
   simp [env_ok_def]
   \\ strip_tac
-  \\ conj_tac
   \\ Cases \\ simp [ml_progTheory.nsLookup_nsBind_compute]
   \\ rw [] \\ gs [SF SFY_ss]
 QED
@@ -743,6 +744,15 @@ Proof
   \\ imp_res_tac STRING_TYPE_perms_ok
   \\ imp_res_tac NUM_perms_ok
   \\ imp_res_tac TERM_TYPE_perms_ok \\ fs []
+QED
+
+(* TODO
+ *)
+Theorem v_ok_Conv_alt:
+  v_ok ctxt (Conv (SOME stamp) vs) ⇒
+    EVERY (v_ok ctxt) vs
+Proof
+  cheat
 QED
 
 val _ = export_theory ();
